tests/lean/run/1675.lean
@@ -8,3 +8,19 @@ begin
   intros h₁ h₂,
   simp_all
 end
+
+example (a b : nat) (p : nat → Prop) (h₁ : a = b + 0) (h₂ : b = 0) (h₃ : p a) : p 0 ∧ a = 0 :=
+by simp_all
+
+constant q : Prop
+axiom q_lemma : q
+
+open tactic
+example (a b : nat) (p : nat → Prop) (h₁ : a = b + 0) (h₂ : b = 0) (h₃ : p a) : p 0 ∧ a = 0 ∧ q :=
+begin
+  simp_all,
+  guard_target q,
+  do {e₁ ← get_local `h₁ >>= infer_type, e₂ ← to_expr ```(a = 0), guard (e₁ = e₂)},
+  do {e₁ ← get_local `h₃ >>= infer_type, e₂ ← to_expr ```(p 0), guard (e₁ = e₂)},
+  apply q_lemma
+end
